term subst

Arithmetization/ISigmaOne/Metamath/Term.lean
@@ -7,21 +7,25 @@ namespace LO.FirstOrder.Arith.Model
 
 variable {M : Type*} [Zero M] [One M] [Add M] [Mul M] [LT M] [M ⊧ₘ* 𝐈𝚺₁]
 
-namespace FormalizedTerm
-
 variable {L : Model.Language M} {pL : LDef} [Model.Language.Defined L pL]
 
-abbrev qqBvar (z : M) : M := ⟪0, z⟫ + 1
+section term
 
-abbrev qqFvar (x : M) : M := ⟪1, x⟫ + 1
+def qqBvar (z : M) : M := ⟪0, z⟫ + 1
 
-abbrev qqFunc (k f v : M) : M := ⟪2, ⟪k, ⟪f, v⟫⟫⟫ + 1
+def qqFvar (x : M) : M := ⟪1, x⟫ + 1
+
+def qqFunc (k f v : M) : M := ⟪2, ⟪k, ⟪f, v⟫⟫⟫ + 1
 
 scoped prefix:max "^#" => qqBvar
 
 scoped prefix:max "^&" => qqFvar
 
 scoped prefix:max "^func " => qqFunc
+
+@[simp] lemma var_lt_qqBvar (z : M) : z < ^#z := lt_succ_iff_le.mpr <| le_pair_right 0 z
+
+@[simp] lemma var_lt_qqFvar (x : M) : x < ^&x := lt_succ_iff_le.mpr <| le_pair_right 1 x
 
 @[simp] lemma arity_lt_qqFunc (k f v : M) : k < ^func k f v :=
   le_iff_lt_succ.mp <| le_trans (le_pair_right 2 k) <| pair_le_pair_right 2 <| le_pair_left k ⟪f, v⟫
@@ -31,6 +35,56 @@ scoped prefix:max "^func " => qqFunc
 
 @[simp] lemma terms_lt_qqFunc (k f v : M) : v < ^func k f v :=
   le_iff_lt_succ.mp <| le_trans (le_pair_right f v) <| le_trans (le_pair_right k ⟪f, v⟫) <| le_pair_right 2 ⟪k, ⟪f, v⟫⟫
+
+lemma lt_qqFunc_of_mem {i b k f v : M} (hi : ⟪i, b⟫ ∈ v) : b < ^func k f v :=
+  _root_.lt_trans (lt_of_mem_rng hi) (terms_lt_qqFunc k f v)
+
+@[simp] lemma qqBvar_inj {z z' : M} : ^#z = ^#z' ↔ z = z' := by simp [qqBvar]
+
+@[simp] lemma qqFvar_inj {x x' : M} : ^&x = ^&x' ↔ x = x' := by simp [qqFvar]
+
+@[simp] lemma qqFunc_inj {k f v k' f' v' : M} : ^func k f v = ^func k' f' v' ↔ k = k' ∧ f = f' ∧ v = v' := by simp [qqFunc]
+
+def _root_.LO.FirstOrder.Arith.qqBvarDef : 𝚺₀-Semisentence 2 := .mkSigma “t z | ∃ t' < t, !pairDef t' 0 z ∧ t = t' + 1” (by simp)
+
+lemma qqBvar_defined : 𝚺₀-Function₁ (qqBvar : M → M) via qqBvarDef := by
+  intro v; simp [qqBvarDef]
+  constructor
+  · intro h; exact ⟨⟪0, v 1⟫, by simp [qqBvar, h], rfl, h⟩
+  · rintro ⟨x, _, rfl, h⟩; exact h
+
+@[simp] lemma eval_qqBvarDef (v) :
+    Semiformula.Evalbm M v qqBvarDef.val ↔ v 0 = ^#(v 1) := qqBvar_defined.df.iff v
+
+def _root_.LO.FirstOrder.Arith.qqFvarDef : 𝚺₀-Semisentence 2 := .mkSigma “t x | ∃ t' < t, !pairDef t' 1 x ∧ t = t' + 1” (by simp)
+
+lemma qqFvar_defined : 𝚺₀-Function₁ (qqFvar : M → M) via qqFvarDef := by
+  intro v; simp [qqFvarDef]
+  constructor
+  · intro h; exact ⟨⟪1, v 1⟫, by simp [qqFvar, h], rfl, h⟩
+  · rintro ⟨x, _, rfl, h⟩; exact h
+
+@[simp] lemma eval_qqFvarDef (v) :
+    Semiformula.Evalbm M v qqFvarDef.val ↔ v 0 = ^&(v 1) := qqFvar_defined.df.iff v
+
+private lemma qqFunc_graph {x k f v : M} :
+    x = ^func k f v ↔ ∃ fv < x, fv = ⟪f, v⟫ ∧ ∃ kfv < x, kfv = ⟪k, fv⟫ ∧ ∃ x' < x, x' = ⟪2, kfv⟫ ∧ x = x' + 1 :=
+  ⟨by rintro rfl
+      exact ⟨⟪f, v⟫, lt_succ_iff_le.mpr <| le_trans (le_pair_right _ _) (le_pair_right _ _), rfl,
+        ⟪k, ⟪f, v⟫⟫, lt_succ_iff_le.mpr <| by simp, rfl,
+        ⟪2, ⟪k, ⟪f, v⟫⟫⟫, by simp [qqFunc], rfl, rfl⟩,
+   by rintro ⟨_, _, rfl, _, _, rfl, _, _, rfl, rfl⟩; rfl⟩
+
+def _root_.LO.FirstOrder.Arith.qqFuncDef : 𝚺₀-Semisentence 4 := .mkSigma
+  “x k f v | ∃ fv < x, !pairDef fv f v ∧ ∃ kfv < x, !pairDef kfv k fv ∧ ∃ x' < x, !pairDef x' 2 kfv ∧ x = x' + 1” (by simp)
+
+lemma qqFunc_defined : 𝚺₀-Function₃ (qqFunc : M → M → M → M) via qqFuncDef := by
+  intro v; simp [qqFuncDef, qqFunc_graph]
+
+@[simp] lemma eval_qqFuncDef (v) :
+    Semiformula.Evalbm M v qqFuncDef.val ↔ v 0 = ^func (v 1) (v 2) (v 3) := qqFunc_defined.df.iff v
+
+namespace FormalizedTerm
 
 variable (L)
 
@@ -57,55 +111,12 @@ private lemma phi_iff (n : M) (C : M) (t : M) :
     · right; right; exact ⟨k, f, v, hkf, Sv, hk,
         fun i u hi ↦ hv i (lt_of_mem_dom hi) u (lt_of_mem_rng hi) hi, rfl⟩
 
-def _root_.LO.FirstOrder.Arith.qqBvarDef : 𝚺₀-Semisentence 2 := .mkSigma “t z | ∃ t' < t, !pairDef t' 0 z ∧ t = t' + 1” (by simp)
-
-lemma qqBvar_defined : 𝚺₀-Function₁ (qqBvar : M → M) via qqBvarDef := by
-  intro v; simp [qqBvarDef]
-  constructor
-  · intro h; exact ⟨⟪0, v 1⟫, by simp [h], rfl, h⟩
-  · rintro ⟨x, _, rfl, h⟩; exact h
-
-@[simp] lemma eval_qqBvarDef (v) :
-    Semiformula.Evalbm M v qqBvarDef.val ↔ v 0 = ^#(v 1) := qqBvar_defined.df.iff v
-
-def _root_.LO.FirstOrder.Arith.qqFvarDef : 𝚺₀-Semisentence 2 := .mkSigma “t x | ∃ t' < t, !pairDef t' 1 x ∧ t = t' + 1” (by simp)
-
-lemma qqFvar_defined : 𝚺₀-Function₁ (qqFvar : M → M) via qqFvarDef := by
-  intro v; simp [qqFvarDef]
-  constructor
-  · intro h; exact ⟨⟪1, v 1⟫, by simp [h], rfl, h⟩
-  · rintro ⟨x, _, rfl, h⟩; exact h
-
-@[simp] lemma eval_qqFvarDef (v) :
-    Semiformula.Evalbm M v qqFvarDef.val ↔ v 0 = ^&(v 1) := qqFvar_defined.df.iff v
-
-private lemma qqFunc_graph {x k f v : M} :
-    x = ^func k f v ↔ ∃ fv < x, fv = ⟪f, v⟫ ∧ ∃ kfv < x, kfv = ⟪k, fv⟫ ∧ ∃ x' < x, x' = ⟪2, kfv⟫ ∧ x = x' + 1 :=
-  ⟨by rintro rfl
-      exact ⟨⟪f, v⟫, lt_succ_iff_le.mpr <| le_trans (le_pair_right _ _) (le_pair_right _ _), rfl,
-        ⟪k, ⟪f, v⟫⟫, lt_succ_iff_le.mpr <| by simp, rfl,
-        ⟪2, ⟪k, ⟪f, v⟫⟫⟫, by simp, rfl, rfl⟩,
-   by rintro ⟨_, _, rfl, _, _, rfl, _, _, rfl, rfl⟩; rfl⟩
-
-def _root_.LO.FirstOrder.Arith.qqFuncDef : 𝚺₀-Semisentence 4 := .mkSigma
-  “x k f v | ∃ fv < x, !pairDef fv f v ∧ ∃ kfv < x, !pairDef kfv k fv ∧ ∃ x' < x, !pairDef x' 2 kfv ∧ x = x' + 1” (by simp)
-
-lemma qqFunc_defined : 𝚺₀-Function₃ (qqFunc : M → M → M → M) via qqFuncDef := by
-  intro v; simp [qqFuncDef, qqFunc_graph]
-
-@[simp] lemma eval_qqFuncDef (v) :
-    Semiformula.Evalbm M v qqFuncDef.val ↔ v 0 = ^func (v 1) (v 2) (v 3) := qqFunc_defined.df.iff v
-
-variable (pL)
-
-def formula : Fixpoint.Formula 1 := ⟨.ofZero (.mkSigma
+def formula (pL : LDef) : Fixpoint.Formula 1 := ⟨.ofZero (.mkSigma
   “t C n |
     (∃ z < n, !qqBvarDef t z) ∨
     (∃ x < t, !qqFvarDef t x) ∨
     (∃ k < t, ∃ f < t, ∃ v < t, !pL.func k f ∧ :Seq v ∧ !lhDef k v ∧ (∀ i < v, ∀ u < v, i ~[v] u → u ∈ C) ∧ !qqFuncDef t k f v)”
   (by simp)) _⟩
-
-variable {pL}
 
 def construction : Fixpoint.Construction M (formula pL) where
   Φ := fun n ↦ Phi L (n 0)
@@ -126,19 +137,23 @@ end FormalizedTerm
 
 open FormalizedTerm
 
-variable (L : Model.Language M) {pL : LDef} [Model.Language.Defined L pL]
+variable (L)
 
 def IsSemiterm (n : M) : M → Prop := (construction L).Fixpoint ![n]
 
-variable (pL)
+def _root_.LO.FirstOrder.Arith.LDef.isSemitermDef (pL : LDef) : 𝚫₁-Semisentence 2 := (formula pL).fixpointDef.rew (Rew.substs ![#1, #0])
 
-def _root_.LO.FirstOrder.Arith.isSemitermDef : 𝚫₁-Semisentence 2 := (formula pL).fixpointDef.rew (Rew.substs ![#1, #0])
-
-variable {pL}
-
-lemma isSemiterm_defined : 𝚫₁-Relation (IsSemiterm L) via (isSemitermDef pL) :=
+lemma isSemiterm_defined : 𝚫₁-Relation (IsSemiterm L) via pL.isSemitermDef :=
   ⟨HSemiformula.ProperOn.rew (construction L).fixpoint_defined.proper _,
-   by intro v; simp [isSemitermDef, (construction L).eval_fixpointDef]; rfl⟩
+   by intro v; simp [LDef.isSemitermDef, (construction L).eval_fixpointDef]; rfl⟩
+
+@[simp] lemma eval_isSemitermDef (v) :
+    Semiformula.Evalbm M v pL.isSemitermDef.val ↔ IsSemiterm L (v 0) (v 1) := (isSemiterm_defined L).df.iff v
+
+instance isSemitermDef_definable : 𝚫₁-Relation (IsSemiterm L) := Defined.to_definable _ (isSemiterm_defined L)
+
+@[simp, definability] instance isSemitermDef_definable' (Γ) : (Γ, m + 1)-Relation (IsSemiterm L) :=
+  .of_deltaOne (isSemitermDef_definable L) _ _
 
 variable {L}
 
@@ -146,22 +161,40 @@ variable {n : M}
 
 local prefix:80 "𝐓ⁿ " => IsSemiterm L n
 
-lemma IsSemiterm.case {t : M} :
+lemma IsSemiterm.case_iff {t : M} :
     𝐓ⁿ t ↔
     (∃ z < n, t = ^#z) ∨
     (∃ x, t = ^&x) ∨
     (∃ k f v : M, L.Func k f ∧ Seq v ∧ k = lh v ∧ (∀ i u, ⟪i, u⟫ ∈ v → 𝐓ⁿ u) ∧ t = ^func k f v) :=
   (construction L).case
 
-lemma IsSemiterm.bvar {z : M} (hz : z < n) : 𝐓ⁿ ^#z := IsSemiterm.case.mpr (Or.inl ⟨z, hz, rfl⟩)
+alias ⟨IsSemiterm.case, IsSemiterm.mk⟩ := IsSemiterm.case_iff
 
-lemma IsSemiterm.fvar (x : M) : 𝐓ⁿ ^&x := IsSemiterm.case.mpr (Or.inr <| Or.inl ⟨x, rfl⟩)
+@[simp] lemma IsSemiterm.bvar {z : M} : 𝐓ⁿ ^#z ↔ z < n :=
+  ⟨by intro h
+      rcases h.case with (⟨z', hz, hzz'⟩ | ⟨x, h⟩ | ⟨k, f, v, _, _, _, _, h⟩)
+      · rcases (show z = z' from by simpa using hzz'); exact hz
+      · simp [qqBvar, qqFvar] at h
+      · simp [qqBvar, qqFunc] at h,
+    fun hz ↦ IsSemiterm.mk (Or.inl ⟨z, hz, rfl⟩)⟩
+
+@[simp] lemma IsSemiterm.fvar (x : M) : 𝐓ⁿ ^&x := IsSemiterm.mk (Or.inr <| Or.inl ⟨x, rfl⟩)
 
 lemma IsSemiterm.func {k f v : M} (hkf : L.Func k f) (Sv : Seq v) (hk : k = lh v)
     (h : ∀ i u, ⟪i, u⟫ ∈ v → 𝐓ⁿ u) :
-    𝐓ⁿ ^func k f v := IsSemiterm.case.mpr (Or.inr <| Or.inr ⟨k, f, v, hkf, Sv, hk, h, rfl⟩)
+    𝐓ⁿ (^func k f v) := IsSemiterm.mk (Or.inr <| Or.inr ⟨k, f, v, hkf, Sv, hk, h, rfl⟩)
 
-lemma IsSemiterm.induction {Γ} {P : M → Prop} (hP : (Γ, 1)-Predicate P)
+lemma IsSemiterm.func_iff {k f v : M} :
+    𝐓ⁿ (^func k f v) ↔ L.Func k f ∧ Seq v ∧ k = lh v ∧ ∀ i u, ⟪i, u⟫ ∈ v → 𝐓ⁿ u :=
+  ⟨by intro h
+      rcases h.case with (⟨_, _, h⟩ | ⟨x, h⟩ | ⟨k', f', v', hkf, Sv, hk, hv, h⟩)
+      · simp [qqFunc, qqBvar] at h
+      · simp [qqFunc, qqFvar] at h
+      · rcases (show k = k' ∧ f = f' ∧ v = v' by simpa [qqFunc] using h) with ⟨rfl, rfl, rfl⟩
+        exact ⟨hkf, Sv, hk, hv⟩,
+   by rintro ⟨hkf, Sv, hk, hv⟩; exact IsSemiterm.func hkf Sv hk hv⟩
+
+lemma IsSemiterm.induction (Γ) {P : M → Prop} (hP : (Γ, 1)-Predicate P)
     (hbvar : ∀ z < n, P (^#z)) (hfvar : ∀ x, P (^&x))
     (hfunc : ∀ k f v, L.Func k f → Seq v → k = lh v → (∀ i u, ⟪i, u⟫ ∈ v → 𝐓ⁿ u ∧ P u) → P (^func k f v)) :
     ∀ t, 𝐓ⁿ t → P t :=
@@ -170,6 +203,240 @@ lemma IsSemiterm.induction {Γ} {P : M → Prop} (hP : (Γ, 1)-Predicate P)
     · exact hbvar z hz
     · exact hfvar x
     · exact hfunc k f v hkf Sv hk (fun i u hi ↦ hC u (h i u hi)))
+
+end term
+
+section termSubst
+
+namespace FormalizedTermSubst
+
+variable (L)
+
+def Phi (n m w : M) (C : Set M) (p : M) : Prop :=
+  IsSemiterm L n (π₁ p) ∧ IsSemiterm L m (π₂ p) ∧
+  ( (∃ z < n, π₁ p = ^#z ∧ ⟪z, π₂ p⟫ ∈ w) ∨
+    (∃ x, π₁ p = ^&x ∧ π₂ p = ^&x) ∨
+    (∃ k f v v', π₁ p = ^func k f v ∧ π₂ p = ^func k f v' ∧ ∀ i u u', ⟪i, u⟫ ∈ v → ⟪i, u'⟫ ∈ v' → ⟪u, u'⟫ ∈ C) )
+
+private lemma phi_iff (n m w C p : M) :
+    Phi L n m w {x | x ∈ C} p ↔
+    ∃ t₁ ≤ p, ∃ t₂ ≤ p, p = ⟪t₁, t₂⟫ ∧ IsSemiterm L n t₁ ∧ IsSemiterm L m t₂ ∧
+    ( (∃ z < n, t₁ = ^#z ∧ ⟪z, t₂⟫ ∈ w) ∨
+      (∃ x < t₁, t₁ = ^&x ∧ t₂ = ^&x) ∨
+      (∃ k < t₁, ∃ f < t₁, ∃ v < t₁, ∃ v' < t₂, t₁ = ^func k f v ∧ t₂ = ^func k f v' ∧
+        (∀ i < v, ∀ u < v, ∀ u' < v', ⟪i, u⟫ ∈ v → ⟪i, u'⟫ ∈ v' → ⟪u, u'⟫ ∈ C)) ) := by
+  constructor
+  ·{intro ⟨hp₁, hp₂, h⟩
+    refine ⟨π₁ p, by simp, π₂ p, by simp, by simp, hp₁, hp₂, ?_⟩
+    rcases h with (⟨z, hz, h₁, h⟩ | ⟨x, h₁, h₂⟩ | ⟨k, f, v, v', h₁, h₂, h⟩)
+    · left; exact ⟨z, hz, h₁, h⟩
+    · right; left; exact ⟨x, by simp [h₁], h₁, h₂⟩
+    · right; right
+      exact ⟨k, by simp [h₁], f, by simp [h₁], v, by simp [h₁], v', by simp [h₂],
+        h₁, h₂, fun i _ u _ u' _ hi hi' ↦ h i u u' hi hi'⟩}
+  · rintro ⟨t₁, _, t₂, _, rfl, ht₁, ht₂, h⟩
+    refine ⟨by simpa using ht₁, by simpa using ht₂, ?_⟩
+    rcases h with (⟨z, hz, rfl, h⟩ | ⟨x, _, rfl, rfl⟩ | ⟨k, _, f, _, v, _, v', _, rfl, rfl, h⟩)
+    · left; exact ⟨z, hz, by simp [h]⟩
+    · right; left; exact ⟨x, by simp⟩
+    · right; right
+      exact ⟨k, f, v, v', by simp, by simp, fun i u u' hi hi' ↦
+        h i (lt_of_mem_dom hi) u (lt_of_mem_rng hi) u' (lt_of_mem_rng hi') hi hi'⟩
+
+def formulaAux : Semisentence ℒₒᵣ 7 := “t₁ t₂ p C n m w |
+  (∃ z < n, !qqBvarDef t₁ z ∧ z ~[w] t₂) ∨
+  (∃ x < t₁, !qqFvarDef t₁ x ∧ !qqFvarDef t₂ x) ∨
+  (∃ k < t₁, ∃ f < t₁, ∃ v < t₁, ∃ v' < t₂, !qqFuncDef t₁ k f v ∧ !qqFuncDef t₂ k f v' ∧
+  (∀ i < v, ∀ u < v, ∀ u' < v', i ~[v] u → i ~[v'] u' → u ~[C] u'))”
+
+def formula (pL : LDef) : Fixpoint.Formula 3 := ⟨.mkDelta
+  (.mkSigma
+    “p C n m w |
+      ∃ t₁ <⁺ p, ∃ t₂ <⁺ p, !pairDef p t₁ t₂ ∧ !pL.isSemitermDef.sigma n t₁ ∧ !pL.isSemitermDef.sigma m t₂ ∧
+      !formulaAux t₁ t₂ p C n m w”
+    (by simp [formulaAux]))
+  (.mkPi
+    “p C n m w |
+      ∃ t₁ <⁺ p, ∃ t₂ <⁺ p, !pairDef p t₁ t₂ ∧ !pL.isSemitermDef.pi n t₁ ∧ !pL.isSemitermDef.pi m t₂ ∧
+      !formulaAux t₁ t₂ p C n m w”
+    (by simp [formulaAux]))⟩
+
+def construction : Fixpoint.Construction M (formula pL) where
+  Φ := fun v ↦ Phi L (v 0) (v 1) (v 2)
+  defined := ⟨fun v ↦
+    by simp [formula, HSemiformula.val_sigma, eval_isSemitermDef L, (isSemiterm_defined L).proper.iff'],
+  fun v ↦ by simpa [formula, HSemiformula.val_sigma, eval_isSemitermDef L, formulaAux] using phi_iff _ _ _ _ _ _⟩
+  monotone := by
+    rintro C C' hC v p ⟨ht₁, ht₂, (h | h | ⟨k, f, v, v', h₁, h₂, h⟩)⟩
+    · exact ⟨ht₁, ht₂, Or.inl h⟩
+    · exact ⟨ht₁, ht₂, Or.inr <| Or.inl h⟩
+    · exact ⟨ht₁, ht₂, Or.inr <| Or.inr ⟨k, f, v, v', h₁, h₂, fun i u u' hi hi' ↦ hC (h i u u' hi hi')⟩⟩
+  finite := by
+    rintro C v p ⟨ht₁, ht₂, (h | h | ⟨k, f, v, v', h₁, h₂, h⟩)⟩
+    · exact ⟨ht₁, ht₂, Or.inl h⟩
+    · exact ⟨ht₁, ht₂, Or.inr <| Or.inl h⟩
+    · exact ⟨ht₁, ht₂, Or.inr <| Or.inr ⟨k, f, v, v', h₁, h₂, fun i u u' hi hi' ↦ ⟨h i u u' hi hi', by
+      have : ⟪u, u'⟫ < ⟪π₁ p, π₂ p⟫ := pair_lt_pair (by simpa [h₁] using lt_qqFunc_of_mem hi) (by simpa [h₂] using lt_qqFunc_of_mem hi')
+      simpa using this⟩⟩⟩
+
+def Rew (n m w : M) : M → Prop := (construction L).Fixpoint ![n, m, w]
+
+def rewDef (pL : LDef) : 𝚫₁-Semisentence 4 := (formula pL).fixpointDef.rew <| Rew.substs ![#3, #0, #1, #2]
+
+lemma rew_defined : 𝚫₁-Relation₄ (Rew L) via (rewDef pL) :=
+  ⟨HSemiformula.ProperOn.rew (construction L).fixpoint_defined.proper _,
+   by intro v; simp [rewDef, (construction L).eval_fixpointDef, Rew]⟩
+
+@[simp] lemma eval_rewDef (v) :
+    Semiformula.Evalbm M v (rewDef pL).val ↔ Rew L (v 0) (v 1) (v 2) (v 3) := (rew_defined L).df.iff v
+
+instance rew_definable : 𝚫₁-Relation₄ (Rew L) := Defined.to_definable _ (rew_defined L)
+
+@[simp, definability] instance rew_definable' (Γ) : (Γ, m + 1)-Relation₄ (Rew L) :=
+  .of_deltaOne (rew_definable L) _ _
+
+variable {L}
+
+lemma Rew.case_iff {n m w p : M} :
+    Rew L n m w p ↔
+    IsSemiterm L n (π₁ p) ∧ IsSemiterm L m (π₂ p) ∧
+    ( (∃ z < n, π₁ p = ^#z ∧ ⟪z, π₂ p⟫ ∈ w) ∨
+      (∃ x, π₁ p = ^&x ∧ π₂ p = ^&x) ∨
+      (∃ k f v v', π₁ p = ^func k f v ∧ π₂ p = ^func k f v' ∧ ∀ i u u', ⟪i, u⟫ ∈ v → ⟪i, u'⟫ ∈ v' → Rew L n m w ⟪u, u'⟫) ) :=
+  (construction L).case
+
+alias ⟨Rew.case, Rew.mk⟩ := Rew.case_iff
+
+lemma Rew.semiterm₁ {n m w t t'} (h : Rew L n m w ⟪t, t'⟫) : IsSemiterm L n t := by simpa using h.case.1
+
+lemma Rew.semiterm₂ {n m w t t'} (h : Rew L n m w ⟪t, t'⟫) : IsSemiterm L m t' := by simpa using h.case.2.1
+
+lemma Rew.bvar {n m w z u : M} (hz : z < n) (hu : IsSemiterm L m u) (h : ⟪z, u⟫ ∈ w) :
+    Rew L n m w ⟪^#z, u⟫ := Rew.mk ⟨by simp [hz], by simpa using hu, Or.inl ⟨z, hz, by simpa using h⟩⟩
+
+lemma Rew.bvar_iff {n m w z u : M} :
+    Rew L n m w ⟪^#z, u⟫ ↔ z < n ∧ IsSemiterm L m u ∧ ⟪z, u⟫ ∈ w :=
+  ⟨by intro h
+      rcases h.case with ⟨_, hu, (⟨z', hz', hzz', h⟩ | ⟨x, h, _⟩ | ⟨k, f, v, v', h, _⟩)⟩
+      · rcases (show z = z' from by simpa using hzz'); exact ⟨hz', by simpa using hu, by simpa using h⟩
+      · simp [qqBvar, qqFvar] at h
+      · simp [qqBvar, qqFunc] at h,
+   by rintro ⟨hz, Hu, h⟩; exact Rew.bvar hz Hu h⟩
+
+@[simp] lemma Rew.fvar {n m w x : M} :
+    Rew L n m w ⟪^&x, ^&x⟫ := Rew.mk ⟨by simp, by simp, Or.inr <| Or.inl ⟨x, by simp⟩⟩
+
+lemma Rew.fvar_iff {n m w x u : M} :
+    Rew L n m w ⟪^&x, u⟫ ↔ u = ^&x := by
+  constructor
+  · intro h
+    rcases h.case with ⟨_, _, (⟨_, _, h, _⟩ | ⟨x', hx', h⟩ | ⟨_, _, _, _, h, _⟩)⟩
+    · simp [qqBvar, qqFvar] at h
+    · rcases (show x = x' from by simpa using hx'); simpa using h
+    · simp [qqFvar, qqFunc] at h
+  · rintro rfl; simp
+
+lemma Rew.func {n m w k f v v' : M}
+    (hkf : L.Func k f)
+    (Sv : Seq v)
+    (hk : k = lh v)
+    (hv : ∀ i u, ⟪i, u⟫ ∈ v → IsSemiterm L n u)
+    (Sv' : Seq v')
+    (hk' : k = lh v')
+    (hv' : ∀ i u', ⟪i, u'⟫ ∈ v' → IsSemiterm L m u')
+    (H : ∀ i u u', ⟪i, u⟫ ∈ v → ⟪i, u'⟫ ∈ v' → Rew L n m w ⟪u, u'⟫) :
+    Rew L n m w ⟪^func k f v, ^func k f v'⟫ :=
+  Rew.mk ⟨
+    by rw [pi₁_pair]; exact IsSemiterm.func hkf Sv hk hv,
+    by rw [pi₂_pair]; exact IsSemiterm.func hkf Sv' hk' hv',
+    Or.inr <| Or.inr ⟨k, f, v, v', by simp, by simp, H⟩⟩
+
+lemma Rew.func' {n m w k f v u : M} (h : Rew L n m w ⟪^func k f v, u⟫) :
+    ∃ v', Seq v' ∧ k = lh v' ∧ (∀ i u u', ⟪i, u⟫ ∈ v → ⟪i, u'⟫ ∈ v' → Rew L n m w ⟪u, u'⟫) ∧ u = ^func k f v' := by
+  rcases h.case with ⟨_, hu, (⟨_, _, h, _⟩ | ⟨x, h, _⟩ | ⟨k', f', v', v'', h₁, h₂, hv⟩)⟩
+  · simp [qqFunc, qqBvar] at h
+  · simp [qqFunc, qqFvar] at h
+  · rcases (show k = k' ∧ f = f' ∧ v = v' by simpa [qqFunc] using h₁) with ⟨rfl, rfl, rfl⟩
+    rcases (show u = ^func k f v'' by simpa using h₂)
+    have : L.Func k f ∧ Seq v'' ∧ k = lh v'' ∧ ∀ i u, ⟪i, u⟫ ∈ v'' → IsSemiterm L m u := by simpa [IsSemiterm.func_iff] using hu
+    rcases this with ⟨_, Sv'', hk'', _⟩
+    exact ⟨v'', Sv'', hk'', hv, rfl⟩
+
+variable (L)
+
+def TermSeq (n m w : M) : Prop := Seq w ∧ n = lh w ∧ ∀ i u, ⟪i, u⟫ ∈ w → IsSemiterm L m u
+
+variable {L}
+
+protected lemma TermSeq.seq {n m w : M} (h : TermSeq L n m w) : Seq w := h.1
+
+protected lemma TermSeq.lh {n m w : M} (h : TermSeq L n m w) : n = lh w := h.2.1
+
+lemma TermSeq.prop {n m w : M} (h : TermSeq L n m w) : ∀ i u, ⟪i, u⟫ ∈ w → IsSemiterm L m u := h.2.2
+
+variable {n m w} (TSw : TermSeq L n m w)
+
+lemma Rew.rng_exists {t : M} (ht : IsSemiterm L n t) : ∃ u, Rew L n m w ⟪t, u⟫ := by
+  apply IsSemiterm.induction 𝚺 ?_ ?_ ?_ ?_ t ht
+  · definability
+  · intro z hz
+    have : ∃ u, ⟪z, u⟫ ∈ w := TSw.seq.exists (show z < lh w by simpa [TSw.lh] using hz)
+    rcases this with ⟨u, hu⟩
+    exact ⟨u, Rew.bvar hz (TSw.prop z u hu) hu⟩
+  · intro x; exact ⟨^&x, by simp⟩
+  · rintro k f v hkf Sv rfl ih
+    have : ∃ v', Seq v' ∧ lh v' = lh v ∧ ∀ i u', ⟪i, u'⟫ ∈ v' → ∀ u, ⟪i, u⟫ ∈ v → Rew L n m w ⟪u, u'⟫ := by
+      have : ∀ i < lh v, ∃ u', ∀ u, ⟪i, u⟫ ∈ v → Rew L n m w ⟪u, u'⟫ := by
+        intro i hi
+        have : IsSemiterm L n (Sv.nth hi) ∧ ∃ u, Rew L n m w ⟪Sv.nth hi, u⟫ := ih i (Sv.nth hi) (by simp)
+        rcases this with ⟨_, u', hu'⟩
+        exact ⟨u', fun u hiuv  ↦ by rcases Sv.nth_uniq hi hiuv; exact hu'⟩
+      exact sigmaOne_skolem_seq
+        (by have : 𝚺₁-Relation fun x y ↦ ∀ u < v, ⟪x, u⟫ ∈ v → Rew L n m w ⟪u, y⟫ := by definability
+            exact this.of_iff fun w ↦ ⟨fun h u _ ↦ h u, fun h u hv ↦ h u (lt_of_mem_rng hv) hv⟩)
+        this
+    rcases this with ⟨v', Sv', hvv', h⟩
+    exact ⟨^func (lh v) f v',
+      Rew.func hkf Sv rfl (fun i u hi ↦ (ih i u hi).1) Sv' (Eq.symm hvv')
+        (fun i u' hi ↦ by
+          have : i < lh v := by simpa [hvv'] using Sv'.lt_lh_of_mem hi
+          exact h i u' hi (Sv.nth this) (by simp) |>.semiterm₂)
+        (fun i u u' hi hi' ↦ h i u' hi' u hi)⟩
+
+lemma Rew.rng_unique
+    {t u₁ u₂ : M} : Rew L n m w ⟪t, u₁⟫ → Rew L n m w ⟪t, u₂⟫ → u₁ = u₂ := by
+  revert u₁ u₂
+  suffices IsSemiterm L n t → ∀ u₁ u₂, Rew L n m w ⟪t, u₁⟫ → Rew L n m w ⟪t, u₂⟫ → u₁ = u₂
+  by intro u₁ u₂ h₁ h₂; exact this h₁.semiterm₁ u₁ u₂ h₁ h₂
+  intro ht
+  apply IsSemiterm.induction 𝚷 ?_ ?_ ?_ ?_ t ht
+  · definability
+  · simp only [bvar_iff, and_imp]
+    intro z _ u₁ u₂ _ _ h₁ _ _ h₂
+    exact TSw.seq.isMapping.uniq h₁ h₂
+  · simp [Rew.fvar_iff]
+  · intro k f v _ Sv hk ih u₁ u₂ h₁ h₂
+    rcases Rew.func' h₁ with ⟨v₁, Sv₁, hk₁, hvv₁, rfl⟩
+    rcases Rew.func' h₂ with ⟨v₂, Sv₂, hk₂, hvv₂, rfl⟩
+    have : v₁ = v₂ := Sv₁.lh_ext Sv₂ (by simp [←hk₁, ←hk₂]) (by
+      intro i x₁ x₂ hxv₁ hxv₂
+      have hi : i < lh v := by simpa [←hk, hk₁] using Sv₁.lt_lh_of_mem hxv₁
+      exact ih i (Sv.nth hi) (by simp) |>.2 _ _ (hvv₁ _ _ _ (Sv.nth_mem hi) hxv₁) (hvv₂ _ _ _ (Sv.nth_mem hi) hxv₂))
+    rw [this]
+/-
+lemma Rew.rng_exists_unique {t : M} (ht : IsSemiterm L n t) : ∃! u, Rew L n m w ⟪t, u⟫ := by
+  rcases Rew.rng_exists Sw hn Hw ht
+-/
+
+end FormalizedTermSubst
+
+open FormalizedTermSubst
+
+variable (L)
+
+
+
+end termSubst
 
 end LO.FirstOrder.Arith.Model
 
